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�© �! (�K10©) ¦�§ux + yuxy = 0���)"

�© �! (�K10©)¦)���Ã.u�gd�Ä¯Kµ
utt = 9uxx, t > 0, 0 < x < +∞,

u|x=0 = 0,

u|t=0 = x, ut|t=0 = 2 sin x, 0 < x < +∞.
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�© n! (�K20©)�	��k.u�Ä¯Kµ
utt = uxx + f(t, x), t > 0, 0 < x < π,

u|x=0 = 0, ux|x=π = 0,

u|t=0 = sin
3

2
x, ut|t=0 = sin

x

2
, 0 < x < π.

1. �f(t, x) = 0�§¦Ñþã½)¯K�)u1(t, x)¶

2. �f(t, x) = sin
x

2
sinωt, ω 6= k +

1

2
, k ∈ N�§¦Ñþã½)¯K�)u2(t, x)¶

3. �Ñ½)¯K¥�§�àg�f(t, x)!>.^�ÚÐ©^��Ôn¿Â"
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�© o! (�K15©)¦)½)¯Kµ
∂u

∂t
=

1

x

∂

∂x

(
x
∂u

∂x

)
+ u, t > 0, 0 < x < 1,

u|x=0k., ux|x=1 = 0,

u|t=0 = ϕ(x), 0 < x < 1.

�© Ê! (�K15©)¦)XeÑt�§�>�¯Kµuxx + uyy + uzz = z, x2 + y2 + z2 < 1,

u|x2+y2+z2=1 = 0.
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�© 8! (�K15©)�«�Ω = {(x, y)|y > x}"
1. ¦«�Ωþ�Ñt�§)|�X>�¯K���¼ê¶

2. ¦)XeÑt�§�)|�X>�¯Kµ∆2u = 0, (x, y) ∈ Ω,

u(x, x) = ϕ(x).
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�© Ô! (�K15©)�	½)¯Kµut = 4uxx + 3u, −∞ < x < +∞, t > 0,

u(0, x) = ϕ(x), −∞ < x < +∞.
1. ¦Ñþã½)¯K�A�Ä�)¶

2. �ϕ(x) = x�§¦)þã½)¯K"
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1. .Ê.d�f∆33���IXe�L�/ª

∆3 =
∂2

∂x2
+

∂2

∂y2
+

∂2

∂z2
=

1

r

∂

∂r

(
r
∂

∂r

)
+

1

r2
∂2

∂θ2
+

∂2

∂z2

=
1

r2
∂

∂r

(
r2
∂

∂r

)
+

1

r2 sin θ

∂

∂θ

(
sin θ

∂

∂θ

)
+

1

r2 sin2 θ

∂2

∂ϕ2
.

2. ��î.�§µx2y′′ + pxy′ + qy = f(x)§3�Cþ��x = et e§�±�z�

~Xê�5�©�§µ
d2y

dt2
+ (p− 1)

dy

dt
+ qy = f(et)"

3. Legendre�§:
[
(1− x2)y′

]′
+ λy = 0; n�Legendreõ�ªµ

Pn(x) =
[n
2
]∑

k=0

(−1)k(2n− 2k)!

2nk!(n− k)!(n− 2k)!
xn−2k =

1

2nn!

dn

dxn
(x2 − 1)n;

Legendreõ�ª�1¼êµ(1 − 2xt + t2)−
1
2 =

∞∑
n=0

Pn(x)tn, |t| < 1; Legendreõ

�ª��²�µ‖Pn(x)‖2 =
2

2n+ 1
.

4. ν�Bessel�§µx2y′′ + xy′ + (x2 − ν2)y = 0; ν�Bessel¼ê:

Jν(x) =
+∞∑
k=0

(−1)k

k!Γ(k + ν + 1)

(x
2

)2k+ν
; Bessel¼ê�1¼êµe

x
2
(ζ−ζ−1) =

+∞∑
n=−∞

Jn(x)ζn;

Bessel¼ê3na>.^�e��²�µN2
ν1n =

a2

2
J2
ν+1(ω1na), N2

ν2n =
1

2
[a2 −

ν2

ω2
2n

]J2
ν (ω2na), N2

ν3n =
1

2
[a2 − ν2

ω2
2n

+
a2α2

β2ω2
3n

]J2
ν (ω3na).

5. Fp�C�Ú_C�: F [f ](λ) =

∫ +∞

−∞
f(x)eiλxdx¶F−1[F ](x) =

1

2π

∫ +∞

−∞
F (λ)e−iλxdλ;

F−1[e−λ2 ] =
1

2
√
π
e−

x2

4 .

6. .Ê.dC�: L[f(t)] =

∫ +∞

0

f(t)e−ptdt, p = σ + is; L[eαt] =
1

p− α
,

L[tα] =
Γ(α + 1)

pα+1
, L[sin t] =

1

p2 + 1
, L[cos t] =

p

p2 + 1
, L[

1√
πt
e−

a2

4t ] =
e−a
√
p

√
p
"

7. .Ê.d�§∆3u = δ(M)�Ä�)µ

��§U(x, y) = − 1

2π
ln

1

r
, r =

√
x2 + y2¶

n�§U(x, y, z) = − 1

4πr
, r =

√
x2 + y2 + z2.
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